

Problem:

Suppose we have a  $3 \times 3$  matrix filled with real numbers in such a way that;

the number in each cell is the sum of the numbers in its neighboring cells.

Prove that- the only solution to this problem is the trivial matrix filled with 0's in all cells that is:

0	0	0
0	0	0
0	0	0

Solution

$x_{11}$	$x_{12}$	$x_{13}$
$x_{21}$	$x_{22}$	$x_{23}$
$x_{31}$	$x_{32}$	$x_{33}$

$$x_{11} = x_{12} + x_{21} + x_{22}$$

$$x_{12} = x_{11} + x_{21} + x_{22} + x_{23} + x_{13}$$

$$x_{13} = x_{12} + x_{22} + x_{23}$$

$$x_{21} = x_{11} + x_{12} + x_{22} + x_{32} + x_{31}$$

$$x_{22} = x_{11} + x_{12} + x_{13} + x_{21} + x_{23} \\ + x_{31} + x_{32} + x_{33}$$

$$x_{23} = x_{13} + x_{12} + x_{22} + x_{32} + x_{33}$$

$$x_{31} = x_{21} + x_{22} + x_{32}$$

$$x_{32} = x_{31} + x_{21} + x_{22} + x_{23} + x_{33}$$

$$x_{33} = x_{32} + x_{22} + x_{23}$$

$$x_{12} = x_{12} + x_{21} + x_{22}$$

$$x_{12} = (x_{12} + x_{21} + x_{22}) + x_{21}$$

$$x_{22} + x_{23} + x_{13}$$

$$2x_{21} + 2x_{22} + x_{23} + x_{13} = 0 \quad \text{--- (1)}$$

$$x_{21} = (x_{12} + x_{21} + x_{22}) + x_{12}$$

$$x_{22} + x_{32} + x_{31}$$

$$2x_{12} + 2x_{22} + x_{32} + x_{31} = 0 \quad \text{--- (2)}$$

$$x_{22} = (x_{11} + x_{33}) + (x_{12} + x_{21})$$

$$+ (x_{13} + x_{23} + x_{32} + x_{31})$$

$$= (x_{12} + x_{21} + x_{22} + x_{32} + x_{23} + x_{22})$$

$$+ (x_{12} + x_{21})$$

$$+ (x_{23} + x_{32})$$

$$+ (x_{13} + x_{31})$$



$$x_{22} = 2x_{22} + 2(x_{12} + x_{21}) + 2(x_{23} + x_{32}) + (x_{13} + x_{31}) \quad \text{--- (3)}$$

$$x_{3/2} = x_{31} + x_{21} + x_{22} + x_{23} + x_{32}$$

$$x_{3/2} + x_{22} + x_{23}$$

$$2x_{23} + 2x_{22} + x_{21} + x_{32} = 0 \quad \text{--- (4)}$$

$$x_{23} = (x_{32} + x_{2/3} + x_{22}) + x_{13} + x_{12} + x_{22} + x_{32}$$

$$2x_{32} + 2x_{22} + x_{13} + x_{12} = 0 \quad \text{--- (5)}$$

Adding (1) & (2) we get,

$$4x_{22} + 2(x_{12} + x_{21}) + x_{23} + (x_{13} + x_{31}) + (x_{23} + x_{32}) = 0 \quad \text{--- (6)}$$

$$4x_{22} + 2(x_{23} + x_{32}) + (x_{12} + x_{21}) + (x_{13} + x_{31}) = 0 \quad \text{--- (7)}$$

$$8x_{22} + 3(x_{12} + x_{21}) + 3(x_{23} + x_{32}) + 2(x_{13} + x_{31}) = 0 \quad \text{--- (8)}$$

$$8x_{22} + \frac{3}{2} \left[ -x_{22} - (x_{13} + x_{31}) \right]$$

$$+ 2(x_{13} + x_{31}) = 0$$

$$\left(8 - \frac{3}{2}\right)x_{22} + \left(2 - \frac{3}{2}\right)(x_{13} + x_{31}) = 0$$

$$15x_{22} + (x_{13} + x_{31}) = 0 \quad \text{--- (9)}$$

$$x_{13} + x_{31} = 2x_{22} + (x_{12} + x_{21}) + (x_{23} + x_{32}) \quad \text{--- (10)}$$

$$x_{13} + x_{31} = 2x_{22} + \frac{1}{2} \left[ -x_{22} - (x_{13} + x_{31}) \right]$$

$$\left(1 + \frac{1}{2}\right)(x_{13} + x_{31}) = \left(2 - \frac{1}{2}\right)x_{22}$$

$$3(x_{13} + x_{31}) = x_{22} \quad \text{--- (11)}$$

(9) & (10) together imply that

$$x_{22} = 0, \quad x_{13} + x_{31} = 0$$

$$\Rightarrow (x_{12} + x_{21}) + (x_{23} + x_{32}) = 0$$

$$\text{--- (12)}$$

$$x_{22} = x_{11} + (x_{12} + x_{21}) + (x_{23} + x_{32}) \\ + (x_{13} + x_{31}) + x_{33}$$

$$\Rightarrow \cancel{0} = \cancel{x_{11} + x_{33}} \\ x_{11} + x_{33} = 0 \quad \text{--- (13)}$$

$$\text{But } \cancel{x_{11} + x_{33}} = \cancel{(x_{12} + x_{21}) + (x_{22} + x_{23})} \\ + \cancel{2x_{22}}$$

$$x_{12} = x_{11} + x_{21} + x_{22} + x_{23} + x_{13}$$

$$\& x_{21} = x_{11} + x_{12} + x_{22} + x_{32} + x_{31}$$

together imply that,

$$(x_{12} + x_{21}) = 2x_{11} + (x_{12} + x_{21}) + 2x_{22} \\ + (x_{23} + x_{32}) + (x_{13} + x_{31})$$

$$\Rightarrow \cancel{2x_{11}} = \cancel{x_{12} + x_{21}} \quad \text{--- (14)}$$

Reduced equation:

$$x_{11} = x_{12} + x_{21} \quad \text{--- (15)}$$

$$x_{13} = x_{12} + x_{23} \quad \text{--- (16)}$$

$$x_{31} = x_{21} + x_{32} \quad \text{--- (17)}$$

$$x_{33} = x_{23} + x_{32} \quad \text{--- (18)}$$



$$\text{let } x_{11} = m \Rightarrow x_{33} = -m$$

$$\text{let } x_{13} = n \Rightarrow x_{31} = -n$$

our matrix now looks like this:

$m$	$x_{12}$	$n$
$x_{21}$	$0$	$x_{23}$
$-n$	$x_{32}$	$-m$

— (\*)

$$x_{12} + x_{21} + 0 = m$$

and  $x_{12} + x_{23} + 0 = n$

$$\Rightarrow 2x_{12} + (x_{21} + x_{23}) = m + n$$

$$\text{But } x_{12} = (x_{21} + x_{23}) + (m+n)$$

$$\Rightarrow 3x_{12} = 2(m+n)$$

$$\Rightarrow x_{12} = \frac{2}{3}(m+n) \quad \text{--- (19)}$$

$$\Rightarrow x_{21} + x_{23} = -\frac{1}{3}(m+n)$$

— (20)

$$\begin{aligned}
 \Rightarrow x_{21} &= m - x_{12} \\
 &= m - \frac{2}{3}(m+n) \\
 &= \frac{1}{3}m - \frac{2}{3}n \quad \text{--- (21)}
 \end{aligned}$$

$$\begin{aligned}
 \& x_{23} &= n - x_{12} \\
 &= \frac{1}{3}n - \frac{2}{3}m \quad \text{--- (22)}
 \end{aligned}$$

(21) implies that

$$\begin{aligned}
 x_{32} &= -n - x_{21} \\
 &= -n - \frac{1}{3}m + \frac{2}{3}n \\
 &= -\frac{1}{3}(m+n) \quad \text{--- (23)}
 \end{aligned}$$

which is also implied by (22).

~~But, by symmetry~~ But

$$x_{21} + x_{32} = -n$$

and,  $x_{23} + x_{32} = -n$

$$\Rightarrow 2x_{32} + (x_{21} + x_{23}) = -(m+n)$$



and,

$$x_{32} - (x_{21} + x_{23}) = -(m+n).$$

$$\Rightarrow 3x_{32} = -2(m+n)$$

$$\Rightarrow x_{32} = -\frac{2}{3}(m+n) \quad \text{--- (24)}$$

comparing (23) & (24) we get,

$$-\frac{2}{3}(m+n) = -\frac{1}{3}(m+n)$$

$$\Rightarrow m+n = 0$$

Now our matrix looks like this:

$$x_{21} \begin{array}{|c|c|c|} \hline m & 0 & -m \\ \hline m & 0 & -m \\ \hline m & 0 & -m \\ \hline \end{array} \quad \text{--- (**)}$$

$$m = x_{21} = m + 0 + 0 + 0 + m$$

$$\Rightarrow m = 2m \Rightarrow m = 0$$

So the only possible solution is

0	0	0
0	0	0
0	0	0

This completes the proof.

$m$	0	$m$
$m$	0	$m$
$m$	0	$m$

$$m + 0 + 0 + 0 = m$$

$$0 = m$$

$$m = m$$